src/proof/k8s_io/apimachinery/pkg/apis/meta/v1.v
@@ -4,10 +4,10 @@ From New.proof Require Import prelude empty_ffi pure_objects.
 Section proof.
 Context `{hG: !heapGS Σ} {go_ctx: GoContext}.
 
-Lemma wp_Now:
+Lemma wp_Now :
   {{{ is_pkg_init v1 }}}
     @! v1.Now #()
-  {{{ (c: v1.Time.t) v, RET #c;
+  {{{ c v, RET #c;
     TimeV.deepown c v
   }}}.
 Proof. Admitted.
@@ -22,6 +22,28 @@ Lemma wp_GetName l m :
   }}}.
 Proof. wp_start as "H". wp_auto. iApply "HΦ". iFrame. Qed.
 
+Lemma wp_GetName_deepown l m :
+  {{{ is_pkg_init v1 ∗
+      ObjectMetaV.deepown_l l m 1
+  }}}
+    l @ (ptrT.id v1.ObjectMeta.id) @ "GetName" #()
+  {{{ RET #m.(ObjectMetaV.Name');
+      ObjectMetaV.deepown_l l m 1
+  }}}.
+Proof.
+  iIntros (Φ) "(#Hinit & Hdeepown_l) HΦ".
+  iDestruct "Hdeepown_l" as (c) "[Hl Hdeepown]".
+  wp_apply (wp_GetName with "[$Hinit $Hl]").
+  iIntros "Hl".
+  iNamed "Hdeepown".
+  rewrite Hdeepown_name.
+  iApply "HΦ".
+  iExists c.
+  iFrame.
+  iPureIntro.
+  done.
+Qed.
+
 Lemma wp_SetName l m name :
   {{{ is_pkg_init v1 ∗
       l ↦ m
@@ -31,6 +53,27 @@ Lemma wp_SetName l m name :
       l ↦ m <| v1.ObjectMeta.Name' := name |>
   }}}.
 Proof. wp_start as "H". wp_auto. iApply "HΦ". iFrame. Qed.
+
+Lemma wp_SetName_deepown l m name :
+  {{{ is_pkg_init v1 ∗
+      ObjectMetaV.deepown_l l m 1
+  }}}
+    l @ (ptrT.id v1.ObjectMeta.id) @ "SetName" #name
+  {{{ RET #();
+      ObjectMetaV.deepown_l l (m <| ObjectMetaV.Name' := name |>) 1
+  }}}.
+Proof.
+  iIntros (Φ) "(#Hinit & Hdeepown_l) HΦ".
+  iDestruct "Hdeepown_l" as (c) "[Hl Hdeepown]".
+  wp_apply (wp_SetName with "[$Hinit $Hl]").
+  iIntros "Hl".
+  iNamed "Hdeepown".
+  iApply "HΦ".
+  iExists (c <| v1.ObjectMeta.Name' := name |>).
+  iFrame.
+  iPureIntro.
+  done.
+Qed.
 
 Lemma wp_GetGenerateName l m :
   {{{ is_pkg_init v1 ∗
@@ -42,6 +85,28 @@ Lemma wp_GetGenerateName l m :
   }}}.
 Proof. wp_start as "H". wp_auto. iApply "HΦ". iFrame. Qed.
 
+Lemma wp_GetGenerateName_deepown l m :
+  {{{ is_pkg_init v1 ∗
+      ObjectMetaV.deepown_l l m 1
+  }}}
+    l @ (ptrT.id v1.ObjectMeta.id) @ "GetGenerateName" #()
+  {{{ RET #m.(ObjectMetaV.GenerateName');
+      ObjectMetaV.deepown_l l m 1
+  }}}.
+Proof.
+  iIntros (Φ) "(#Hinit & Hdeepown_l) HΦ".
+  iDestruct "Hdeepown_l" as (c) "[Hl Hdeepown]".
+  wp_apply (wp_GetGenerateName with "[$Hinit $Hl]").
+  iIntros "Hl".
+  iNamed "Hdeepown".
+  rewrite Hdeepown_generatename.
+  iApply "HΦ".
+  iExists c.
+  iFrame.
+  iPureIntro.
+  done.
+Qed.
+
 Lemma wp_SetNamespace l m namespace :
   {{{ is_pkg_init v1 ∗
       l ↦ m
@@ -52,6 +117,27 @@ Lemma wp_SetNamespace l m namespace :
   }}}.
 Proof. wp_start as "H". wp_auto. iApply "HΦ". iFrame. Qed.
 
+Lemma wp_SetNamespace_deepown l m namespace :
+  {{{ is_pkg_init v1 ∗
+      ObjectMetaV.deepown_l l m 1
+  }}}
+    l @ (ptrT.id v1.ObjectMeta.id) @ "SetNamespace" #namespace
+  {{{ RET #();
+      ObjectMetaV.deepown_l l (m <| ObjectMetaV.Namespace' := namespace |>) 1
+  }}}.
+Proof.
+  iIntros (Φ) "(#Hinit & Hdeepown_l) HΦ".
+  iDestruct "Hdeepown_l" as (c) "[Hl Hdeepown]".
+  wp_apply (wp_SetNamespace with "[$Hinit $Hl]").
+  iIntros "Hl".
+  iNamed "Hdeepown".
+  iApply "HΦ".
+  iExists (c <| v1.ObjectMeta.Namespace' := namespace |>).
+  iFrame.
+  iPureIntro.
+  done.
+Qed.
+
 Lemma wp_SetCreationTimestamp l m creation_timestamp :
   {{{ is_pkg_init v1 ∗
       l ↦ m
@@ -61,6 +147,28 @@ Lemma wp_SetCreationTimestamp l m creation_timestamp :
       l ↦ m <| v1.ObjectMeta.CreationTimestamp' := creation_timestamp |>
   }}}.
 Proof. wp_start as "H". wp_auto. iApply "HΦ". iFrame. Qed.
+
+Lemma wp_SetCreationTimestamp_deepown l m creation_timestamp pure_creation_timestamp :
+  {{{ is_pkg_init v1 ∗
+      ObjectMetaV.deepown_l l m 1 ∗
+      TimeV.deepown creation_timestamp pure_creation_timestamp
+  }}}
+    l @ (ptrT.id v1.ObjectMeta.id) @ "SetCreationTimestamp" #creation_timestamp
+  {{{ RET #();
+      ObjectMetaV.deepown_l l (m <| ObjectMetaV.CreationTimestamp' := pure_creation_timestamp |>) 1
+  }}}.
+Proof.
+  iIntros (Φ) "(#Hinit & Hdeepown_l & Hdeepown_time) HΦ".
+  iDestruct "Hdeepown_l" as (c) "[Hl Hdeepown]".
+  wp_apply (wp_SetCreationTimestamp with "[$Hinit $Hl]").
+  iIntros "Hl".
+  iNamed "Hdeepown".
+  iApply "HΦ".
+  iExists (c <| v1.ObjectMeta.CreationTimestamp' := creation_timestamp |>).
+  iFrame.
+  iPureIntro.
+  done.
+Qed.
 
 Lemma wp_GetDeletionTimestamp l m :
   {{{ is_pkg_init v1 ∗
@@ -82,6 +190,32 @@ Lemma wp_SetDeletionTimestamp l m deletion_timestamp :
   }}}.
 Proof. wp_start as "H". wp_auto. iApply "HΦ". iFrame. Qed.
 
+Lemma wp_SetDeletionTimestamp_deepown l m deletion_timestamp pure_deletion_timestamp :
+  {{{ is_pkg_init v1 ∗
+      ObjectMetaV.deepown_l l m 1 ∗
+      ⌜ deletion_timestamp = null ↔ pure_deletion_timestamp = None ⌝ ∗
+      (match pure_deletion_timestamp with
+       | Some vd => ∃ cd, deletion_timestamp ↦ cd ∗ TimeV.deepown cd vd
+       | None => True
+       end)
+  }}}
+    l @ (ptrT.id v1.ObjectMeta.id) @ "SetDeletionTimestamp" #deletion_timestamp
+  {{{ RET #();
+      ObjectMetaV.deepown_l l (m <| ObjectMetaV.DeletionTimestamp' := pure_deletion_timestamp |>) 1
+  }}}.
+Proof.
+  iIntros (Φ) "(#Hinit & Hdeepown_l & %Hdeletiontimestamp_none & Hdeletiontimestamp_some) HΦ".
+  iDestruct "Hdeepown_l" as (c) "[Hl Hdeepown]".
+  wp_apply (wp_SetDeletionTimestamp with "[$Hinit $Hl]").
+  iIntros "Hl".
+  iNamed "Hdeepown".
+  iApply "HΦ".
+  iExists (c <| v1.ObjectMeta.DeletionTimestamp' := deletion_timestamp |>).
+  iFrame.
+  iPureIntro.
+  done.
+Qed.
+
 Lemma wp_SetDeletionGracePeriodSeconds l m deletion_grace_period_seconds :
   {{{ is_pkg_init v1 ∗
       l ↦ m
@@ -91,6 +225,33 @@ Lemma wp_SetDeletionGracePeriodSeconds l m deletion_grace_period_seconds :
       l ↦ m <| v1.ObjectMeta.DeletionGracePeriodSeconds' := deletion_grace_period_seconds |>
   }}}.
 Proof. wp_start as "H". wp_auto. iApply "HΦ". iFrame. Qed.
+
+Lemma wp_SetDeletionGracePeriodSeconds_deepown
+    l m deletion_grace_period_seconds pure_deletion_grace_period_seconds :
+  {{{ is_pkg_init v1 ∗
+      ObjectMetaV.deepown_l l m 1 ∗
+      ⌜ deletion_grace_period_seconds = null ↔ pure_deletion_grace_period_seconds = None ⌝ ∗
+      (match pure_deletion_grace_period_seconds with
+       | Some vd => ∃ cd, deletion_grace_period_seconds ↦ cd ∗ ⌜ cd = vd ⌝
+       | None => True
+       end)
+  }}}
+    l @ (ptrT.id v1.ObjectMeta.id) @ "SetDeletionGracePeriodSeconds" #deletion_grace_period_seconds
+  {{{ RET #();
+      ObjectMetaV.deepown_l l (m <| ObjectMetaV.DeletionGracePeriodSeconds' := pure_deletion_grace_period_seconds |>) 1
+  }}}.
+Proof.
+  iIntros (Φ) "(#Hinit & Hdeepown_l & %Hdeletion_grace_period_seconds_none & Hdeletion_grace_period_seconds_some) HΦ".
+  iDestruct "Hdeepown_l" as (c) "[Hl Hdeepown]".
+  wp_apply (wp_SetDeletionGracePeriodSeconds with "[$Hinit $Hl]").
+  iIntros "Hl".
+  iNamed "Hdeepown".
+  iApply "HΦ".
+  iExists (c <| v1.ObjectMeta.DeletionGracePeriodSeconds' := deletion_grace_period_seconds |>).
+  iFrame.
+  iPureIntro.
+  done.
+Qed.
 
 Lemma wp_SetSelfLink l m self_link :
   {{{ is_pkg_init v1 ∗
@@ -102,6 +263,27 @@ Lemma wp_SetSelfLink l m self_link :
   }}}.
 Proof. wp_start as "H". wp_auto. iApply "HΦ". iFrame. Qed.
 
+Lemma wp_SetSelfLink_deepown l m self_link :
+  {{{ is_pkg_init v1 ∗
+      ObjectMetaV.deepown_l l m 1
+  }}}
+    l @ (ptrT.id v1.ObjectMeta.id) @ "SetSelfLink" #self_link
+  {{{ RET #();
+      ObjectMetaV.deepown_l l (m <| ObjectMetaV.SelfLink' := self_link |>) 1
+  }}}.
+Proof.
+  iIntros (Φ) "(#Hinit & Hdeepown_l) HΦ".
+  iDestruct "Hdeepown_l" as (c) "[Hl Hdeepown]".
+  wp_apply (wp_SetSelfLink with "[$Hinit $Hl]").
+  iIntros "Hl".
+  iNamed "Hdeepown".
+  iApply "HΦ".
+  iExists (c <| v1.ObjectMeta.SelfLink' := self_link |>).
+  iFrame.
+  iPureIntro.
+  done.
+Qed.
+
 Lemma wp_SetResourceVersion l m resource_version :
   {{{ is_pkg_init v1 ∗
       l ↦ m
@@ -111,6 +293,27 @@ Lemma wp_SetResourceVersion l m resource_version :
       l ↦ m <| v1.ObjectMeta.ResourceVersion' := resource_version |>
   }}}.
 Proof. wp_start as "H". wp_auto. iApply "HΦ". iFrame. Qed.
+
+Lemma wp_SetResourceVersion_deepown l m resource_version :
+  {{{ is_pkg_init v1 ∗
+      ObjectMetaV.deepown_l l m 1
+  }}}
+    l @ (ptrT.id v1.ObjectMeta.id) @ "SetResourceVersion" #resource_version
+  {{{ RET #();
+      ObjectMetaV.deepown_l l (m <| ObjectMetaV.ResourceVersion' := resource_version |>) 1
+  }}}.
+Proof.
+  iIntros (Φ) "(#Hinit & Hdeepown_l) HΦ".
+  iDestruct "Hdeepown_l" as (c) "[Hl Hdeepown]".
+  wp_apply (wp_SetResourceVersion with "[$Hinit $Hl]").
+  iIntros "Hl".
+  iNamed "Hdeepown".
+  iApply "HΦ".
+  iExists (c <| v1.ObjectMeta.ResourceVersion' := resource_version |>).
+  iFrame.
+  iPureIntro.
+  done.
+Qed.
 
 Lemma wp_GetFinalizers l m :
   {{{ is_pkg_init v1 ∗
@@ -131,6 +334,27 @@ Lemma wp_SetUID l m uid :
       l ↦ m <| v1.ObjectMeta.UID' := uid |>
   }}}.
 Proof. wp_start as "H". wp_auto. iApply "HΦ". iFrame. Qed.
+
+Lemma wp_SetUID_deepown l m uid :
+  {{{ is_pkg_init v1 ∗
+      ObjectMetaV.deepown_l l m 1
+  }}}
+    l @ (ptrT.id v1.ObjectMeta.id) @ "SetUID" #uid
+  {{{ RET #();
+      ObjectMetaV.deepown_l l (m <| ObjectMetaV.UID' := uid |>) 1
+  }}}.
+Proof.
+  iIntros (Φ) "(#Hinit & Hdeepown_l) HΦ".
+  iDestruct "Hdeepown_l" as (c) "[Hl Hdeepown]".
+  wp_apply (wp_SetUID with "[$Hinit $Hl]").
+  iIntros "Hl".
+  iNamed "Hdeepown".
+  iApply "HΦ".
+  iExists (c <| v1.ObjectMeta.UID' := uid |>).
+  iFrame.
+  iPureIntro.
+  done.
+Qed.
 
 Definition new_controller_ref_valid controller_ref kind m : Prop :=
   controller_ref.(OwnerReferenceV.Kind') = kind ∧
